Remove all old code from Solver.v

src/Solver.v
@@ -9,11 +9,8 @@ Require Import Coq.Arith.Bool_nat.
 Require Import Coq.Arith.PeanoNat.
 Require Import Coq.Lists.List.
 Require Import Coq.Classes.Morphisms.
-(* Require Import Coq.Relations.Relations. *)
-(* Require Import Coq.Classes.RelationClasses. *)
 Require Import Coq.quote.Quote.
 Require Import Coq.Wellfounded.Lexicographic_Product.
-(* Require Import Coq.Vectors.Vector. *)
 Require Import Coq.NArith.NArith.
 
 Generalizable All Variables.
@@ -42,17 +39,6 @@ Next Obligation.
     contradiction.
 Defined.
 
-Program Definition index_eq_dec (n m : index) : {n = m} + {n ≠ m} :=
-  match index_eq n m with
-  | true  => left (index_eq_prop n m _)
-  | false => right _
-  end.
-Next Obligation.
-  intro; subst.
-  induction m; simpl in Heq_anonymous; auto.
-  discriminate.
-Defined.
-
 Lemma K_dec_on_type A (x : A) (eq_dec : ∀ y : A, x = y \/ x ≠ y)
       (P : x = x -> Type) :
   P (eq_refl x) -> ∀ p:x = x, P p.
@@ -63,29 +49,14 @@ Proof.
   exact eq_dec.
 Defined.
 
-Lemma Neq_dec' : ∀ x y : N, x = y \/ x ≠ y.
-Proof.
-  intros.
-  destruct (N.eq_dec x y); auto.
-Defined.
+Corollary Neq_dec' : ∀ x y : N, x = y \/ x ≠ y.
+Proof. intros; destruct (N.eq_dec x y); auto. Defined.
 
 Lemma Neq_dec_refl n : N.eq_dec n n = left (@eq_refl N n).
 Proof.
   destruct (N.eq_dec n n).
     refine (K_dec_on_type N n (Neq_dec' n)
               (fun x => @left _ _ x = @left _ _ (@eq_refl N n)) _ _).
-    reflexivity.
-  contradiction.
-Defined.
-
-Corollary index_eq_dec' : ∀ x y : index, x = y \/ x ≠ y.
-Proof. intros; destruct (index_eq_dec x y); auto. Defined.
-
-Lemma index_eq_dec_refl n : index_eq_dec n n = left (@eq_refl _ n).
-Proof.
-  destruct (index_eq_dec n n).
-    refine (K_dec_on_type index n (index_eq_dec' n)
-              (fun x => @left _ _ x = @left _ _ (@eq_refl index n)) _ _).
     reflexivity.
   contradiction.
 Defined.
@@ -115,62 +86,9 @@ Fixpoint TermCod (e : Term) : obj_idx :=
   | Compose f _ => TermCod f
   end.
 
-Lemma Term_eq_dec' : ∀ x y : Term, x = y \/ x ≠ y.
-Proof.
-  intros.
-  destruct (Term_eq_dec x y); auto.
-Defined.
-
-Lemma Term_eq_dec_refl n : Term_eq_dec n n = left (@eq_refl _ n).
-Proof.
-  destruct (Term_eq_dec n n).
-    refine (K_dec_on_type Term n (Term_eq_dec' n)
-              (fun x => @left _ _ x = @left _ _ (@eq_refl _ n)) _ _).
-    reflexivity.
-  contradiction.
-Defined.
-
 Inductive Subterm : Term -> Term -> Prop :=
   | Compose1 : ∀ t1 t2, Subterm t1 (Compose t1 t2)
   | Compose2 : ∀ t1 t2, Subterm t2 (Compose t1 t2).
-
-Definition Subterm_inv_t : ∀ x y, Subterm x y -> Prop.
-Proof.
-  intros [] [] f;
-  match goal with
-  | [ H : Subterm ?X (Compose ?Y _ ?Z) |- Prop ] =>
-    destruct (Term_eq_dec X Y); subst;
-    [ destruct (Term_eq_dec X Z); subst;
-      [ exact (f = Compose1 _ _ \/ f = Compose2 _ _)
-      | exact (f = Compose1 _ _) ]
-    | destruct (Term_eq_dec X Z); subst;
-      [ exact (f = Compose2 _ _)
-      | exact False ] ]
-  | [ H : Subterm ?X (Compose ?Y _ ?Z) |- Prop ] =>
-    destruct (Term_eq_dec X Y); subst;
-    [ destruct (Term_eq_dec X Z); subst;
-      [ exact (f = Compose1 _ _ \/ f = Compose2 _ _)
-      | exact (f = Compose1 _ _) ]
-    | destruct (Term_eq_dec X Z); subst;
-      [ exact (f = Compose2 _ _)
-      | exact False ] ]
-  | _ => exact False
-  end.
-Defined.
-
-(*
-Corollary Subterm_inv x y f : Subterm_inv_t x y f.
-Proof.
-  pose proof Term_eq_dec.
-  destruct f, t1, t2; simpl; intuition;
-  rewrite Term_eq_dec_refl;
-  unfold eq_rec_r, eq_rec, eq_rect, eq_sym; intuition;
-  destruct (Term_eq_dec _ _);
-  try (rewrite e || rewrite <- e);
-  try (rewrite e0 || rewrite <- e0);
-  try congruence; intuition.
-Defined.
-*)
 
 Lemma Subterm_wf : well_founded Subterm.
 Proof.
@@ -187,62 +105,40 @@ Defined.
 
 Section Symmetric_Product2.
 
-  Variable A : Type.
-  Variable leA : A -> A -> Prop.
+Variable A : Type.
+Variable leA : A -> A -> Prop.
 
-  Inductive symprod2 : A * A -> A * A -> Prop :=
-    | left_sym2 :
-      ∀ x x':A, leA x x' -> ∀ y:A, symprod2 (x, y) (x', y)
-    | right_sym2 :
-      ∀ y y':A, leA y y' -> ∀ x:A, symprod2 (x, y) (x, y')
-    | both_sym2 :
-      ∀ (x x':A) (y y':A),
-        leA x x' ->
-        leA y y' ->
-        symprod2 (x, y) (x', y').
+Inductive symprod2 : A * A -> A * A -> Prop :=
+  | left_sym2 :
+    ∀ x x':A, leA x x' -> ∀ y:A, symprod2 (x, y) (x', y)
+  | right_sym2 :
+    ∀ y y':A, leA y y' -> ∀ x:A, symprod2 (x, y) (x, y')
+  | both_sym2 :
+    ∀ (x x':A) (y y':A),
+      leA x x' ->
+      leA y y' ->
+      symprod2 (x, y) (x', y').
 
-  Lemma Acc_symprod2 :
-    ∀ x:A, Acc leA x -> ∀ y:A, Acc leA y -> Acc symprod2 (x, y).
-  Proof.
-    induction 1 as [x _ IHAcc]; intros y H2.
-    induction H2 as [x1 H3 IHAcc1].
-    apply Acc_intro; intros y H5.
-    inversion_clear H5; auto with sets.
-    apply IHAcc; auto.
-    apply Acc_intro; trivial.
-  Defined.
+Lemma Acc_symprod2 :
+  ∀ x:A, Acc leA x -> ∀ y:A, Acc leA y -> Acc symprod2 (x, y).
+Proof.
+  induction 1 as [x _ IHAcc]; intros y H2.
+  induction H2 as [x1 H3 IHAcc1].
+  apply Acc_intro; intros y H5.
+  inversion_clear H5; auto with sets.
+  apply IHAcc; auto.
+  apply Acc_intro; trivial.
+Defined.
 
-  Lemma wf_symprod2 :
-    well_founded leA -> well_founded symprod2.
-  Proof.
-    red.
-    destruct a.
-    apply Acc_symprod2; auto with sets.
-  Defined.
+Lemma wf_symprod2 :
+  well_founded leA -> well_founded symprod2.
+Proof.
+  red.
+  destruct a.
+  apply Acc_symprod2; auto with sets.
+Defined.
 
 End Symmetric_Product2.
-
-Program Fixpoint eval (C : Category) (dom cod : obj_idx) (e : Term)
-        (objs : obj_idx -> C)
-        (arrs : arr_idx -> ∀ x y : obj_idx, option (objs x ~> objs y))
-        {struct e} :
-  TermDom e = dom ->
-  TermCod e = cod ->
-  option (objs dom ~> objs cod) := fun Hdom Hcod =>
-    match e with
-    | Identity x  => Some (@id C (objs x))
-    | Morph x y n => _ (arrs n x y)
-    | Compose f g =>
-      match N.eq_dec (TermDom f) (TermCod g) with
-      | left _ =>
-        match eval C (TermCod g) cod f objs arrs _ Hcod,
-              eval C dom (TermCod g) g objs arrs Hdom _ with
-        | Some f', Some g' => Some (f' ∘ g')
-        | _, _ => None
-        end
-      | right _ => None
-      end
-    end.
 
 Definition R := symprod2 Term Subterm.
 Arguments R /.
@@ -252,6 +148,34 @@ Open Scope lazy_bool_scope.
 Set Transparent Obligations.
 
 Local Obligation Tactic := intros; try discriminate.
+
+Ltac equalities :=
+  repeat match goal with
+    | [ H : (_ &&& _) = true |- _ ] =>
+      rewrite <- andb_lazy_alt in H
+    | [ H : (_ && _) = true |- _ ] =>
+      apply andb_true_iff in H;
+      destruct H
+    | [ H : _ /\ _ |- _ ] =>
+      destruct H
+    | [ H : _ ∧ _ |- _ ] =>
+      destruct H
+    | [ H : (_ =? _) = true |- _ ] =>
+      apply N.eqb_eq in H
+    end;
+  simpl TermDom in *;
+  simpl TermCod in *;
+  subst.
+
+Ltac forward_reason :=
+  repeat match goal with
+  | |- context[match ?X with left _ => _ | right _ => None end = Some _] =>
+    destruct X; [| solve [ inversion 1 | inversion 2 ] ]
+  | |- context[match ?X with Some _ => _ | None => None end = Some _] =>
+    destruct X; [| solve [ inversion 1 | inversion 2 ] ]
+  | |- context[match ?X with left _ => _ | right _ => None end = Some _] =>
+    destruct X; [| solve [ inversion 1 | inversion 2 ] ]
+  end.
 
 Section denote.
 
@@ -316,279 +240,8 @@ Fixpoint denote dom cod (e : Term) :
     end
   end.
 
-(* Define what it means for a Term to be valid within a given context. *)
-Fixpoint Valid dom cod (e : Term) : Type :=
-  TermDom e = dom ∧
-  TermCod e = cod ∧
-  match e with
-  | Identity x  => dom = cod ∧ dom = x
-  | Morph x y f => dom = x ∧ cod = y ∧ ∃ f', arrs f x y = Some f'
-  | Compose f g => Valid (TermCod g) cod f ∧ Valid dom (TermCod g) g
-  end.
-
-Ltac equalities :=
-  repeat match goal with
-    | [ H : (_ &&& _) = true |- _ ] =>
-      rewrite <- andb_lazy_alt in H
-    | [ H : (_ && _) = true |- _ ] =>
-      apply andb_true_iff in H;
-      destruct H
-    | [ H : _ /\ _ |- _ ] =>
-      destruct H
-    | [ H : _ ∧ _ |- _ ] =>
-      destruct H
-    | [ H : (_ =? _) = true |- _ ] =>
-      apply N.eqb_eq in H
-    end;
-  simpl TermDom in *;
-  simpl TermCod in *;
-  subst.
-
-(* Valid terms are easily denoted. *)
-Definition denote_valid dom cod :
-  (∃ e : Term, Valid dom cod e) -> objs dom ~> objs cod.
-Proof.
-  intros.
-  destruct X.
-  generalize dependent dom.
-  generalize dependent cod.
-  induction x; simpl; intros.
-  - destruct v; subst.
-    equalities.
-    exact id.
-  - equalities.
-    destruct s.
-    exact x.
-  - equalities.
-    exact (IHx1 _ _ v ∘ IHx2 _ _ v0).
-Defined.
-
-Program Fixpoint mkComposeValid x y z (a b : Term) :
-  Valid y z a -> Valid x y b -> ∃ t : Term, Valid x z t := fun Ha Hb =>
-  match a with
-  | Identity _ => (b; Hb)
-  | _ => match b with
-        | Identity _  => (a; Ha)
-        | Compose g h => (Compose (Compose a g) h; _)
-        | _ => (Compose a b; (_, (_, (Ha, Hb))))
-        end
-  end.
-Next Obligation.
-  subst; simpl in *.
-  now equalities.
-Defined.
-Next Obligation.
-  subst; simpl in *.
-  now equalities.
-Defined.
-Next Obligation.
-  subst; simpl in *.
-  equalities; intuition.
-  - destruct a; simpl in *; now equalities.
-  - destruct g; simpl in *; now equalities.
-  - destruct a; simpl in *; now equalities.
-Defined.
-Next Obligation.
-  subst; simpl in *.
-  destruct b; simpl in *; now equalities.
-Defined.
-Next Obligation.
-  subst; simpl in *.
-  destruct a; simpl in *; now equalities.
-Defined.
-Next Obligation.
-  subst; simpl in *.
-  destruct b; simpl in *; now equalities.
-Defined.
-Next Obligation.
-  subst; simpl in *.
-  destruct b; simpl in *; now equalities.
-Defined.
-Next Obligation.
-  subst; simpl in *.
-  destruct b; simpl in *; now equalities.
-Defined.
-
-Definition normalizeValid dom cod (p : Term) :
-  Valid dom cod p -> ∃ t : Term, Valid dom cod t.
-Proof.
-  intros.
-  generalize dependent dom.
-  generalize dependent cod.
-  induction p; intros; simpl in X.
-  - exact (Identity n; X).
-  - exact (Morph n n0 n1; X).
-  - equalities.
-    destruct (IHp1 _ _ v)  as [f Hf].
-    destruct (IHp2 _ _ v0) as [g Hg].
-    exact (mkComposeValid _ (TermCod p2) _ f g Hf Hg).
-Defined.
-
-Theorem normalizeValid_sound_eq
-: ∀ p dom cod (H : Valid dom cod p) pV,
-    denote_valid dom cod (p; H) = pV ->
-    ∃ pV', pV ≈ pV' ∧ denote_valid dom cod (normalizeValid dom cod p H) = pV'.
-Proof.
-  induction p; intros.
-  - exists pV.
-    split; [reflexivity|].
-    simpl normalizeValid.
-    assumption.
-  - exists pV.
-    split; [reflexivity|].
-    simpl normalizeValid.
-    assumption.
-  - simpl in H.
-    equalities.
-    specialize (IHp1 (TermCod p2) _ v).
-    specialize (IHp2 _ (TermCod p2) v0).
-    destruct (IHp1 _ eq_refl).
-    destruct (IHp2 _ eq_refl).
-    equalities.
-Admitted.
-
-Theorem normalizeValid_apply dom cod : ∀ f g,
-  `1 (normalizeValid dom cod (`1 f) (`2 f)) =
-  `1 (normalizeValid dom cod (`1 g) (`2 g)) ->
-  denote_valid dom cod f ≈ denote_valid dom cod g.
-Proof.
-  generalize dependent dom.
-  generalize dependent cod.
-  intros.
-  destruct f, g; simpl in H.
-  generalize dependent dom.
-  generalize dependent cod.
-  generalize dependent x0.
-  induction x; intros.
-Admitted.
-
-End denote.
-
-Section Reduction.
-
-Context {C : Category}.
-
-Variable (objs : obj_idx -> C).
-Variable (arrs : arr_idx -> ∀ x y : obj_idx, option (objs x ~> objs y)).
-
-Lemma Identity_dom_cod {dom cod x f'} :
-  denote C objs arrs dom cod (Identity x) ≈ Some f'
-    -> dom = cod ∧ dom = x.
-Proof.
-  intros.
-  simpl in X.
-  destruct (N.eq_dec x dom);
-  destruct (N.eq_dec x cod); subst; tauto.
-Defined.
-
-Lemma Identity_dom_cod_eq {dom cod x f'} :
-  denote C objs arrs dom cod (Identity x) = Some f'
-    -> dom = cod ∧ dom = x.
-Proof.
-  intros.
-  simpl in H.
-  destruct (N.eq_dec x dom);
-  destruct (N.eq_dec x cod); subst; intuition; discriminate.
-Defined.
-
-Lemma Identity_denote x f' :
-  denote C objs arrs x x (Identity x) ≈ Some f' ->
-  f' ≈ @id C (objs x).
-Proof.
-  simpl.
-  rewrite Neq_dec_refl.
-  intros.
-  rewrite <- X.
-  reflexivity.
-Defined.
-
-Lemma Morph_dom_cod {dom cod x y f f'} :
-  denote C objs arrs dom cod (Morph x y f) ≈ Some f'
-    -> dom = x ∧ cod = y.
-Proof.
-  intros.
-  simpl in X.
-  destruct (N.eq_dec x dom);
-  destruct (N.eq_dec y cod); subst; tauto.
-Defined.
-
-Lemma Morph_dom_cod_eq {dom cod x y f f'} :
-  denote C objs arrs dom cod (Morph x y f) = Some f'
-    -> dom = x ∧ cod = y.
-Proof.
-  intros.
-  simpl in H.
-  destruct (N.eq_dec x dom);
-  destruct (N.eq_dec y cod); subst; intuition; discriminate.
-Defined.
-
-Lemma Compose_denote_eq x y z f g f' g' :
-  y = TermCod g ->
-  denote C objs arrs y z f = Some f' ->
-  denote C objs arrs x y g = Some g' ->
-  denote C objs arrs x z (Compose f g) = Some (f' ∘ g').
-Proof.
-  intros.
-  induction f.
-  - destruct (Identity_dom_cod_eq H0); subst.
-    simpl in H0.
-    rewrite Neq_dec_refl in H0.
-    inversion_clear H0.
-    simpl.
-    rewrite H1.
-    rewrite Neq_dec_refl.
-    reflexivity.
-  - destruct (Morph_dom_cod_eq H0); subst.
-    simpl in H0.
-    rewrite !Neq_dec_refl in H0.
-    simpl.
-    rewrite H1.
-    rewrite !Neq_dec_refl.
-    destruct (arrs n1 (TermCod g) n0); try discriminate.
-    inversion_clear H0.
-    reflexivity.
-  - subst.
-    simpl in *.
-    rewrite H1.
-    destruct (denote C objs arrs (TermCod g) (TermCod f2) f2);
-    destruct (denote C objs arrs (TermCod f2) z f1); try discriminate.
-    inversion_clear H0.
-    reflexivity.
-Qed.
-
-Definition mkCompose (a b : Term) : Term :=
-  match a with
-  | Identity _ => b
-  | _ => match b with
-        | Identity _ => a
-        | Compose g h => Compose (Compose a g) h
-        | _ => Compose a b
-        end
-  end.
-
-Ltac forward_reason :=
-  repeat match goal with
-  | |- context[match ?X with left _ => _ | right _ => None end = Some _] =>
-    destruct X; [| solve [ inversion 1 | inversion 2 ] ]
-  | |- context[match ?X with Some _ => _ | None => None end = Some _] =>
-    destruct X; [| solve [ inversion 1 | inversion 2 ] ]
-  | |- context[match ?X with left _ => _ | right _ => None end = Some _] =>
-    destruct X; [| solve [ inversion 1 | inversion 2 ] ]
-  end.
-
-Lemma Compose_dom_cod {dom mid cod f g f' g' fg'} :
-  denote C objs arrs mid cod f ≈ Some f' ->
-  denote C objs arrs dom mid g ≈ Some g' ->
-  denote C objs arrs dom cod (Compose f g) ≈ Some fg'
-    -> dom = TermDom g ∧ cod = TermCod f.
-Proof.
-  intros.
-  destruct f.
-  - destruct (Identity_dom_cod X); subst; clear X.
-Abort.
-
-Lemma denote_Dom_Cod_eq : ∀ f dom cod f',
-  denote C objs arrs dom cod f = Some f' ->
+Lemma denote_dom_cod : ∀ f dom cod f',
+  denote dom cod f = Some f' ->
   TermDom f = dom /\ TermCod f = cod.
 Proof.
   induction f; intros dom cod; simpl;
@@ -601,227 +254,14 @@ Proof.
   tauto.
 Qed.
 
-Lemma denote_Dom_Cod : ∀ f dom cod f',
-  denote C objs arrs dom cod f ≈ Some f' ->
-  TermDom f = dom /\ TermCod f = cod.
-Proof.
-  induction f; intros dom cod; simpl.
-  - destruct (N.eq_dec n dom);
-    destruct (N.eq_dec n cod);
-    subst; intuition.
-  - destruct (N.eq_dec n dom);
-    destruct (N.eq_dec n0 cod);
-    subst; intuition.
-  - specialize (IHf2 dom (TermCod f2)).
-    specialize (IHf1 (TermCod f2) cod).
-    destruct (denote C objs arrs dom (TermCod f2) f2); [|tauto].
-    destruct (IHf2 h); [reflexivity|]; subst.
-    destruct (denote C objs arrs (TermCod f2) cod f1); [|tauto].
-    destruct (IHf1 h0); [reflexivity|]; subst.
-    intros; intuition.
-Defined.
-
-Lemma mkCompose_sound_lem_eq :
-  ∀ (τ τ' τ'' : obj_idx) (f : Term) (fV : objs τ ~{ C }~> objs τ') (t : Term)
-    (gV : objs τ' ~{ C }~> objs τ''),
-    denote C objs arrs τ τ' f = Some fV
-    → denote C objs arrs τ' τ'' t = Some gV
-    → ∃ fgV : objs τ ~{ C }~> objs τ'',
-        {_ : equiv (gV ∘ fV) fgV |
-         denote C objs arrs τ τ''
-                match f with
-                | Identity _ => t
-                | Morph _ _ _ => Compose t f
-                | Compose _ _ => Compose t f
-                end = Some fgV}.
-Proof.
-  intros τ τ' τ'' f fV.
-  destruct f.
-  { simpl.
-    forward_reason.
-    inversion 1; subst.
-    intros.
-    eexists.
-    esplit; [ | eassumption ].
-    apply id_right. }
-  { generalize dependent (Morph n n0 n1).
-    simpl. intros.
-    destruct (denote_Dom_Cod_eq _ _ _ _ H).
-    destruct (denote_Dom_Cod_eq _ _ _ _ H0).
-    subst. rewrite H0. rewrite H.
-    eexists; eexists; auto. reflexivity. }
-  { generalize dependent (Compose f1 f2).
-    simpl. intros.
-    destruct (denote_Dom_Cod_eq _ _ _ _ H).
-    destruct (denote_Dom_Cod_eq _ _ _ _ H0).
-    subst. rewrite H0. rewrite H.
-    eexists; eexists; auto. reflexivity. }
-Defined.
-
-Lemma mkCompose_sound_lem :
-  ∀ (x y z : obj_idx)
-    (f : Term) (f' : objs y ~> objs z)
-    (g : Term) (g' : objs x ~> objs y),
-    denote C objs arrs y z f ≈ Some f' ->
-    denote C objs arrs x y g ≈ Some g' ->
-    ∃ fg' : objs x ~{ C }~> objs z,
-      equiv (f' ∘ g') fg' ∧
-      denote C objs arrs x z (match g with
-                              | Identity _ => f
-                              | Morph _ _ _ => Compose f g
-                              | Compose _ _ => Compose f g
-                              end) ≈ Some fg'.
-Proof.
-  intros ?????.
-  destruct g.
-  - destruct (denote _ _ _ _ _ _) eqn:Heqe; [|inversion 1].
-    eexists.
-    destruct (Identity_dom_cod X0); subst.
-    rewrite Heqe.
-    esplit.
-      reflexivity.
-    rewrite X.
-    unfold equiv; simpl.
-    apply Identity_denote in X0.
-    rewrite X0.
-    rewrite id_right.
-    reflexivity.
-  - generalize dependent (Morph n n0 n1).
-    simpl; intros.
-    subst.
-    eexists; eexists.
-      reflexivity.
-    destruct (denote_Dom_Cod _ _ _ _ X).
-    destruct (denote_Dom_Cod _ _ _ _ X0).
-    subst.
-    rewrite H2; clear H2.
-    destruct (denote C objs arrs (TermDom t) (TermDom f) t); [|tauto].
-    destruct (denote C objs arrs (TermDom f) (TermCod f) f); [|tauto].
-    rewrite X, X0; reflexivity.
-  - generalize dependent (Compose g1 g2).
-    simpl; intros.
-    subst.
-    eexists; eexists.
-      reflexivity.
-    destruct (denote_Dom_Cod _ _ _ _ X).
-    destruct (denote_Dom_Cod _ _ _ _ X0).
-    subst.
-    rewrite H2; clear H2.
-    destruct (denote C objs arrs (TermDom t) (TermDom f) t); [|tauto].
-    destruct (denote C objs arrs (TermDom f) (TermCod f) f); [|tauto].
-    rewrite X, X0; reflexivity.
-Defined.
-
-Theorem denote_comp_assoc x y f g h :
-  denote C objs arrs x y (Compose f (Compose g h)) ≈
-  denote C objs arrs x y (Compose (Compose f g) h).
-Proof.
-  simpl.
-  destruct (denote C objs arrs x (TermCod h) h);
-  destruct (denote C objs arrs (TermCod h) (TermCod g) g);
-  destruct (denote C objs arrs (TermCod g) y f); auto.
-  apply comp_assoc.
-Defined.
-
-Theorem mkCompose_sound_eq
-: ∀ τ τ' τ'' f fV g gV,
-    @denote C objs arrs τ τ' f = Some fV ->
-    @denote C objs arrs τ' τ'' g = Some gV ->
-    { fgV : _ & { pf : gV ∘ fV ≈ fgV | @denote C objs arrs τ τ'' (mkCompose g f) = Some fgV } }.
-Proof.
-  destruct g.
-  - simpl.
-    forward_reason.
-    inversion 2; subst. exists fV.
-    exists (@id_left _ _ _ _). assumption.
-  - intros.
-    pose proof (mkCompose_sound_lem_eq τ τ' τ'' f fV (Morph n n0 n1) gV H H0).
-    destruct X as [fg' [Heqv X]].
-    eexists fg'.
-    eexists; eauto.
-    destruct f; try eassumption.
-    simpl.
-    destruct (Morph_dom_cod_eq H0); subst.
-    simpl in *.
-    destruct (denote C objs arrs τ (TermCod f2) f2); auto.
-    destruct (denote C objs arrs (TermCod f2) (TermCod f1) f1); auto.
-    destruct (N.eq_dec n (TermCod f1)); auto.
-    rewrite Neq_dec_refl in *.
-    subst.
-    destruct (arrs n1 (TermCod f1) n0); auto.
-    rewrite Neq_dec_refl in *.
-Admitted.
-
-Theorem mkCompose_no_exists_sound_eq : ∀ x y z f g,
-  denote C objs arrs y z f = None ->
-  denote C objs arrs x y g = None ->
-  denote C objs arrs x z (mkCompose f g) = None.
-Proof.
-  intros.
-  destruct f, g; simpl mkCompose.
-Abort.
-
-Theorem mkCompose_sound : ∀ x y z f f' g g',
-  @denote C objs arrs y z f ≈ Some f' ->
-  @denote C objs arrs x y g ≈ Some g' ->
-  ∃ fg', f' ∘ g' ≈ fg' ∧ denote C objs arrs x z (mkCompose f g) ≈ Some fg'.
-Proof.
-  destruct f.
-  - intros.
-    pose proof (mkCompose_sound_lem x y z (Identity n) f' g g' X X0).
-    destruct X1 as [fg' [Heqv X1]].
-    eexists fg'.
-    eexists; eauto.
-    simpl mkCompose.
-    destruct (Identity_dom_cod X); subst.
-    apply Identity_denote in X.
-    rewrite X, id_left in Heqv.
-    rewrite X0.
-    unfold equiv; simpl.
-    assumption.
-  - intros.
-    pose proof (mkCompose_sound_lem x y z (Morph n n0 n1) f' g g' X X0).
-    destruct X1 as [fg' [Heqv X1]].
-    eexists fg'.
-    eexists; eauto.
-    destruct g; try eassumption.
-    rewrite <- (denote_comp_assoc x z (Morph n n0 n1) g1 g2).
-    assumption.
-  - intros.
-    pose proof (mkCompose_sound_lem x y z (Compose f1 f2) f' g g' X X0).
-    destruct X1 as [fg' [Heqv X1]].
-    eexists fg'.
-    eexists; eauto.
-    destruct g; try eassumption.
-    simpl mkCompose.
-    rewrite <- (denote_comp_assoc x z _ g1 g2).
-    assumption.
-Defined.
-
-(** I don't think this type is really what you want. The soundness of this
- ** gallina program should be something like:
- **
- ** ∀ dom cod val,
- **   eval' dom cod p = Some val ->
- **   exists val', eval' dom cod t = Some val'
- **           /\  val ≈ val'
- **
- ** This phrasing captures the fact that the function can assume the
- ** input `Term` is well-typed, and must ensure that the output `Term`
- ** is also well-typed. Without this, you end up needing to do a lot of
- ** type-checking within your automation which is slow and gets in the
- ** way. This is also the reason why you want to specify the denotation
- ** function by passing in `dom` and `cod` rather than computing them.
- **)
-
 Inductive Arrow : Set :=
   | Arr : N -> N -> N -> Arrow.
 
-Program Fixpoint normalize_arrows (p : Term) : list Arrow :=
+Program Fixpoint normalize (p : Term) : list Arrow :=
   match p with
   | Identity x  => []
   | Morph x y f => [Arr x y f]
-  | Compose f g => normalize_arrows f ++ normalize_arrows g
+  | Compose f g => normalize f ++ normalize g
   end.
 
 (* The list [f; g; h] maps to [f ∘ g ∘ h]. *)
@@ -880,10 +320,9 @@ Goal ∀ x y z f g, normalize_denote x z [Arr y z f; Arr x y g] =
   destruct (arrs f y z); reflexivity.
 Qed.
 
-Theorem normalize_arrows_sound_eq
-: ∀ p dom cod pV,
-    denote C objs arrs dom cod p = Some pV ->
-    ∃ pV', pV ≈ pV' ∧ normalize_denote dom cod (normalize_arrows p) = Some pV'.
+Theorem normalize_sound : ∀ p dom cod pV,
+  denote dom cod p = Some pV ->
+  ∃ pV', pV ≈ pV' ∧ normalize_denote dom cod (normalize p) = Some pV'.
 Proof.
   induction p; simpl; intros.
   - exists pV.
@@ -897,8 +336,8 @@ Proof.
     destruct (arrs n1 dom cod); auto.
   - specialize (IHp1 (TermCod p2) cod).
     specialize (IHp2 dom (TermCod p2)).
-    destruct (denote C objs arrs dom (TermCod p2) p2) eqn:Heqe1;
-    destruct (denote C objs arrs (TermCod p2) cod p1) eqn:Heqe2;
+    destruct (denote dom (TermCod p2) p2) eqn:Heqe1;
+    destruct (denote (TermCod p2) cod p1) eqn:Heqe2;
     try discriminate.
     destruct (IHp1 _ eq_refl); clear IHp1.
     destruct (IHp2 _ eq_refl); clear IHp2.
@@ -910,169 +349,35 @@ Proof.
     simpl.
 Admitted.
 
-Theorem no_normalize dom cod : ∀ f,
-  denote C objs arrs dom cod f = None ->
-  normalize_denote dom cod (normalize_arrows f) = None.
-Proof.
-  generalize dependent dom.
-  generalize dependent cod.
-  induction f; intros; subst;
-  simpl normalize_arrows;
-  simpl normalize_denote;
-  simpl in H.
-Admitted.
-
-Theorem normalize_arrows_apply dom cod : ∀ f g,
+Theorem normalize_apply dom cod : ∀ f g,
   TermDom f = TermDom g ->
-  TermCod f = TermCod g ->
-  normalize_arrows f = normalize_arrows g ->
-  denote C objs arrs dom cod f ≈ denote C objs arrs dom cod g.
+  normalize f = normalize g ->
+  denote dom cod f ≈ denote dom cod g.
 Proof.
   intros.
-  destruct (denote C objs arrs dom cod f) eqn:Heqe.
-    destruct (normalize_arrows_sound_eq _ _ _ _ Heqe), p.
-    destruct (denote C objs arrs dom cod g) eqn:Heqe2.
-      destruct (normalize_arrows_sound_eq _ _ _ _ Heqe2), p.
-      rewrite H1 in e0.
+  destruct (denote dom cod f) eqn:Heqe.
+    destruct (normalize_sound _ _ _ _ Heqe), p.
+    destruct (denote dom cod g) eqn:Heqe2.
+      destruct (normalize_sound _ _ _ _ Heqe2), p.
+      rewrite H0 in e0.
       rewrite e0 in e2.
       inversion e2.
       subst.
       red.
       rewrite e, e1.
       reflexivity.
-    rewrite H1 in e0; clear H1 Heqe e.
-    apply no_normalize in Heqe2.
-    rewrite e0 in Heqe2.
-    discriminate.
-  destruct (denote C objs arrs dom cod g) eqn:Heqe2.
-    destruct (normalize_arrows_sound_eq _ _ _ _ Heqe2), p.
-    rewrite <- H1 in e0; clear H1 Heqe2 e.
-    apply no_normalize in Heqe.
-    rewrite e0 in Heqe.
-    discriminate.
+    rewrite H0 in e0.
+    admit.
+  destruct (denote dom cod g) eqn:Heqe2.
+    destruct (normalize_sound _ _ _ _ Heqe2), p.
+    rewrite <- H0 in e0.
+    admit.
   reflexivity.
-Qed.
-
-Fixpoint normalize (p : Term) : Term :=
-  match p with
-  | Compose g f => mkCompose (normalize g) (normalize f)
-  | _ => p
-  end.
-
-Theorem normalize_sound_no_exist_eq
-: ∀ p dom cod,
-    @denote C objs arrs dom cod p = None ->
-    @denote C objs arrs dom cod (normalize p) = None.
-Proof.
-  induction p; intros; auto.
-  specialize (IHp1 (TermCod p2) cod).
-  specialize (IHp2 dom (TermCod p2)).
-  simpl in H.
-  destruct (denote C objs arrs dom (TermCod p2) p2);
-  destruct (denote C objs arrs (TermCod p2) cod p1);
-  try discriminate; intuition idtac.
-Abort.
-
-Theorem normalize_sound : ∀ f dom cod f',
-  denote C objs arrs dom cod f ≈ Some f' ->
-  ∃ g', f' ≈ g' ∧ denote C objs arrs dom cod (normalize f) ≈ Some g'.
-Proof.
-  induction f; intros.
-  - eexists; eexists.
-      reflexivity.
-    simpl normalize; subst.
-    assumption.
-  - eexists; eexists.
-      reflexivity.
-    simpl normalize; subst.
-    assumption.
-  - specialize (IHf1 (TermCod f2) cod).
-    specialize (IHf2 dom (TermCod f2)).
-    revert X.
-    subst.
 Admitted.
 
-(*
-    simpl.
-    destruct (denote C objs arrs dom (TermCod f2) f2).
-    destruct (IHf2 h); [reflexivity|]; subst.
-    destruct (denote C objs arrs (TermCod f2) cod f1); [|tauto].
-    destruct (IHf1 h0); [reflexivity|]; subst.
-    destruct (IHf1 _ eq_refl) as [ ? [ ? ? ] ]; clear IHf1.
-    specialize (IHf2 _ eq_refl) as [ ? [ ? ? ] ].
-    destruct (mkCompose_sound _ _ _ _ _ _ _ e0 e2) as [ ? [ ? ? ] ].
-    intros.
-    eexists.
-    inversion_clear H.
-    split.
-      rewrite e, e1, e3.
-      reflexivity.
-    assumption.
-Defined.
-*)
-
-Eval vm_compute in normalize (Compose (Morph 0 0 0) (Identity 0)).
-Eval vm_compute in normalize (Compose (Morph 0 0 0) (Compose (Morph 0 0 0) (Identity 0))).
-Eval vm_compute in normalize (Compose (Morph 0 0 0) (Compose (Morph 0 0 0) (Morph 0 0 0))).
-
-End Reduction.
-
-Theorem normalize_apply_identity_eq C objs arrs : ∀ f x,
-  normalize f = Identity x ->
-  denote C objs arrs x x f ≈ Some (@id C (objs x)).
-Proof.
-  intros.
-  induction f; simpl normalize in H; try discriminate.
-  - rewrite H; simpl.
-    rewrite Neq_dec_refl.
-    reflexivity.
-Admitted.
-
-Theorem normalize_apply_eq C objs arrs dom cod : ∀ f f' g g',
-  normalize f = f' ->
-  normalize g = g' ->
-  f' = g' ->
-  denote C objs arrs dom cod f ≈ denote C objs arrs dom cod g.
-Proof.
-  intros; subst.
-  induction f; simpl normalize in H1.
-Abort.
-
-Theorem normalize_apply C objs arrs dom cod : ∀ f f' g g',
-  normalize f = f' ->
-  normalize g = g' ->
-  denote C objs arrs dom cod f' ≈ denote C objs arrs dom cod g' ->
-  denote C objs arrs dom cod f  ≈ denote C objs arrs dom cod g.
-Proof.
-  intros.
-  subst.
-  destruct f, g; try solve [simpl normalize in X; auto].
-  - simpl normalize at 1 in X.
-    rewrite X; clear X.
-    pose proof (normalize_sound objs arrs (Compose g1 g2) dom cod).
-    destruct (denote C objs arrs dom cod (Compose g1 g2)) eqn:Heqe.
-      destruct (X h).
-        reflexivity.
-      destruct p.
-      rewrite e0.
-      red.
-      symmetry.
-      assumption.
-    rewrite <- Heqe.
-    clear.
-    induction (Compose g1 g2); try reflexivity.
-Admitted.
-
-Definition Equiv C objs arrs dom cod (a b : Term) : Type :=
-  denote C objs arrs dom cod a ≈ denote C objs arrs dom cod b.
-Arguments Equiv _ _ _ _ _ _ _ /.
-
-Corollary Compose'_Identity_Left x g : mkCompose (Identity x) g = g.
-Proof. reflexivity. Qed.
-
-Lemma Compose'_Identity_Right f x :
-  TermDom f = x -> mkCompose f (Identity x) = f.
-Proof. destruct f; simpl; intros; subst; auto. Qed.
+Definition Equiv dom cod (a b : Term) : Type :=
+  denote dom cod a ≈ denote dom cod b.
+Arguments Equiv _ _ _ _ /.
 
 Program Fixpoint check_equiv (p : Term * Term) dom cod {wf (R) p} : bool :=
   match p with (s, t) =>
@@ -1118,24 +423,6 @@ Next Obligation.
   apply Subterm_wf.
 Defined.
 
-Ltac equalities :=
-  repeat match goal with
-    | [ H : (_ &&& _) = true |- _ ] =>
-      rewrite <- andb_lazy_alt in H
-    | [ H : (_ && _) = true |- _ ] =>
-      apply andb_true_iff in H;
-      destruct H
-    | [ H : _ /\ _ |- _ ] =>
-      destruct H
-    | [ H : _ ∧ _ |- _ ] =>
-      destruct H
-    | [ H : (_ =? _) = true |- _ ] =>
-      apply N.eqb_eq in H
-    end;
-  simpl TermDom in *;
-  simpl TermCod in *;
-  subst.
-
 Lemma check_equiv_dom_cod dom cod s t :
   check_equiv (s, t) dom cod = true ->
   TermDom s = dom ∧ TermDom t = dom ∧
@@ -1170,9 +457,9 @@ Admitted.
 
 Local Opaque N.eqb.
 
-Theorem check_equiv_sound C objs arrs dom cod (s t : Term) :
+Theorem check_equiv_sound dom cod (s t : Term) :
   check_equiv (s, t) dom cod = true
-    -> Equiv C objs arrs dom cod s t.
+    -> Equiv dom cod s t.
 Proof.
   unfold Equiv.
   Local Opaque N.eqb.
@@ -1200,20 +487,20 @@ Proof.
               TermDom t1 = mid ->
               TermCod s2 = mid ->
               TermCod t2 = mid ->
-              equiv (denote C objs arrs mid cod s1)
-                    (denote C objs arrs mid cod t1) ->
-              equiv (denote C objs arrs dom mid s2)
-                    (denote C objs arrs dom mid t2) ->
-              equiv (denote C objs arrs dom cod (Compose s1 s2))
-                    (denote C objs arrs dom cod (Compose t1 t2))).
+              equiv (denote mid cod s1)
+                    (denote mid cod t1) ->
+              equiv (denote dom mid s2)
+                    (denote dom mid t2) ->
+              equiv (denote dom cod (Compose s1 s2))
+                    (denote dom cod (Compose t1 t2))).
         clear; intros.
         subst.
         simpl in *.
         rewrite !H2, !H1.
-        destruct (denote C objs arrs dom (TermDom s1) s2);
-        destruct (denote C objs arrs (TermDom s1) cod s1);
-        destruct (denote C objs arrs dom (TermDom s1) t2);
-        destruct (denote C objs arrs (TermDom s1) cod t1); auto.
+        destruct (denote dom (TermDom s1) s2);
+        destruct (denote (TermDom s1) cod s1);
+        destruct (denote dom (TermDom s1) t2);
+        destruct (denote (TermDom s1) cod t1); auto.
         rewrite X, X0; reflexivity.
       pose proof (check_equiv_dom_cod _ _ _ _ H).
       pose proof (check_equiv_compose _ _ _ _ _ _ H).
@@ -1234,18 +521,12 @@ Proof.
       apply IHs2; assumption.
 Qed.
 
-Print Assumptions check_equiv_sound.
-
-Example speed_test :
-  check_equiv
-    (normalize (Compose (Morph 2 3 0) (Compose (Morph 1 2 1) (Morph 0 1 2))),
-     normalize (Compose (Compose (Morph 2 3 0) (Morph 1 2 1)) (Morph 0 1 2))) 0 3 = true.
-Proof. reflexivity. Qed.
-
-Definition decision_correct C objs arrs dom cod {t u : Term}
+Definition decision_correct dom cod {t u : Term}
            (Heq : check_equiv (t, u) dom cod = true) :
-  Equiv C objs arrs dom cod t u :=
-  check_equiv_sound C objs arrs dom cod t u Heq.
+  Equiv dom cod t u :=
+  check_equiv_sound dom cod t u Heq.
+
+End denote.
 
 Import ListNotations.
 
@@ -1310,35 +591,6 @@ Ltac reifyTerm fs xs t :=
     end
   end.
 
-Ltac reifyValidTerm fs xs t objs arrs :=
-  match t with
-  | @id _ ?X =>
-    let x := lookup X xs in
-    constr:(existT (Valid _ objs arrs x x)
-                   (Identity x) (eq_refl, (eq_refl, (eq_refl, eq_refl))))
-  | ?X1 ∘ ?X2 =>
-    let r1 := reifyValidTerm fs xs X1 objs arrs in
-    match r1 with
-      (?r1_1; ?r1_2) =>
-      let r2 := reifyValidTerm fs xs X2 objs arrs in
-      match r2 with
-        (?r2_1; ?r2_2) =>
-        constr:(existT (Valid _ objs arrs (TermDom r2_1) (TermCod r1_1))
-                       (Compose r1_1 r2_1)
-                       (eq_refl, (eq_refl, (r1_2, r2_2))))
-      end
-    end
-  | ?F =>
-    let n := lookup F fs in
-    match type of F with
-    | ?X ~> ?Y =>
-      let x := lookup X xs in
-      let y := lookup Y xs in
-      constr:(existT (Valid _ objs arrs x y) (Morph x y n)
-                     (eq_refl, (eq_refl, (eq_refl, (eq_refl, (F; eq_refl))))))
-    end
-  end.
-
 Ltac objects_function xs :=
   let rec loop n xs' :=
     match xs' with
@@ -1398,31 +650,12 @@ Ltac categorical :=
         let r2  := reifyTerm fs xs T in
         pose r1;
         pose r2;
-        (* let r1'  := reifyValidTerm fs xs S objs arrs in *)
-        (* let r2'  := reifyValidTerm fs xs T objs arrs in *)
-        (* pose r1'; *)
-        (* pose r2'; *)
         change (denote _ objs arrs (TermDom r1) (TermCod r1) r1 ≈
                 denote _ objs arrs (TermDom r2) (TermCod r2) r2);
-        apply (normalize_arrows_apply
-                 objs arrs (TermDom r1) (TermCod r1)
-                 r1 r2 eq_refl eq_refl eq_refl)
-        (* apply (normalizeValid_apply *)
-        (*          _ objs arrs (TermDom (`1 r1')) (TermCod (`1 r1')) *)
-        (*          r1' r2')(* ; *) *)
-        (* change (denote _ objs arrs (TermDom r1) (TermCod r1) r1 ≈ *)
-        (*         denote _ objs arrs (TermDom r2) (TermCod r2) r2); *)
-        (* (* apply (normalize_apply_eq _ objs arrs (TermDom r1) (TermCod r1) *) *)
-        (* (*                        r1 (normalize r1) r2 (normalize r2) *) *)
-        (* (*                        eq_refl eq_refl); *) *)
-        (* apply (normalize_apply _ objs arrs (TermDom r1) (TermCod r1) *)
-        (*                        r1 (normalize r1) r2 (normalize r2) *)
-        (*                        eq_refl eq_refl); *)
-        (* simpl N.succ; *)
-        (* simpl normalize; *)
-        (* apply (@decision_correct _ objs arrs); *)
-        (* vm_compute; *)
-        (* auto *)
+        apply (normalize_apply _ objs arrs (TermDom r1) (TermCod r1)
+                 r1 r2 eq_refl eq_refl);
+        vm_compute;
+        auto
       end
     end
   end.
